safechecker/theories/PCUICWfEnvImpl.v
@@ -6,46 +6,6 @@ From MetaCoq.PCUIC Require Import PCUICAst PCUICAstUtils PCUICEquality PCUICRedu
 From MetaCoq.SafeChecker Require Import PCUICEqualityDec PCUICWfEnv.
 From Equations Require Import Equations.
 
-Lemma wf_gc_of_uctx {cf:checker_flags} {Σ : global_env} (HΣ : ∥ wf Σ ∥)
-: ∑ uctx', gc_of_uctx (global_uctx Σ) = Some uctx'.
-Proof.
-assert (consistent (global_uctx Σ).2) as HC.
-{ sq; apply (wf_consistent _ HΣ). }
-unfold gc_of_uctx; simpl in *.
-apply gc_consistent_iff in HC.
-destruct (gc_of_constraints (global_constraints Σ)).
-eexists; reflexivity.
-contradiction HC.
-Defined.
-
-Lemma graph_of_wf {cf:checker_flags} {Σ : global_env} (HΣ : ∥ wf Σ ∥)
-: ∑ G, is_graph_of_uctx G (global_uctx Σ).
-Proof.
-destruct (wf_gc_of_uctx HΣ) as [uctx Huctx].
-exists (make_graph uctx). unfold is_graph_of_uctx. now rewrite Huctx.
-Defined.
-
-Lemma wf_ext_gc_of_uctx {cf:checker_flags} {Σ : global_env_ext} (HΣ : ∥ wf_ext Σ ∥)
-: ∑ uctx', gc_of_uctx (global_ext_uctx Σ) = Some uctx'.
-Proof.
-assert (consistent (global_ext_uctx Σ).2) as HC.
-{ sq; apply (global_ext_uctx_consistent _ HΣ). }
-destruct Σ as [Σ φ].
-simpl in HC.
-unfold gc_of_uctx; simpl in *.
-apply gc_consistent_iff in HC.
-destruct (gc_of_constraints (global_ext_constraints (Σ, φ))).
-eexists; reflexivity.
-contradiction HC.
-Defined.
-
-Lemma graph_of_wf_ext {cf:checker_flags} {Σ : global_env_ext} (HΣ : ∥ wf_ext Σ ∥)
-: ∑ G, is_graph_of_uctx G (global_ext_uctx Σ).
-Proof.
-destruct (wf_ext_gc_of_uctx HΣ) as [uctx Huctx].
-exists (make_graph uctx). unfold is_graph_of_uctx. now rewrite Huctx.
-Defined.
-
 Class abstract_guard_impl :=
   { guard_impl : FixCoFix -> global_env_ext -> context -> mfixpoint term -> bool ;
     guard_correct : forall fix_cofix Σ Γ mfix, guard fix_cofix Σ Γ mfix <-> guard_impl fix_cofix Σ Γ mfix
@@ -68,27 +28,6 @@ Record referenced_impl {cf:checker_flags} := {
       referenced_impl_graph_wf := projT2 (graph_of_wf referenced_impl_wf)
   }.
 
-Definition check_conv_pb_relb_correct {cf:checker_flags} (Σ : global_env_ext) (HΣ : ∥ wf_ext Σ ∥) G
-  (HG : is_graph_of_uctx G (global_ext_uctx Σ)) conv_pb u u' :
-  wf_universe Σ u' -> wf_universe Σ u ->
-  compare_universe conv_pb Σ u u' <-> conv_pb_relb G conv_pb u u'.
-Proof.
-  intros.  sq.  destruct conv_pb; split; cbn; intro.
-  - apply (check_eqb_universe_complete _ (global_ext_levels Σ, global_ext_constraints Σ)); eauto.
-      + eapply wf_ext_global_uctx_invariants; eauto.
-      + eapply wf_ext_consistent; eauto.
-  - apply (check_eqb_universe_spec' G (global_ext_levels Σ, global_ext_constraints Σ)); eauto.
-      + eapply wf_ext_global_uctx_invariants; eauto.
-      + eapply wf_ext_consistent; eauto.
-  - apply (check_leqb_universe_complete _ (global_ext_levels Σ, global_ext_constraints Σ)); eauto.
-      + eapply wf_ext_global_uctx_invariants; eauto.
-      + eapply wf_ext_consistent; eauto.
-  - apply (check_leqb_universe_spec' G (global_ext_levels Σ, global_ext_constraints Σ)); eauto.
-      + eapply wf_ext_global_uctx_invariants; eauto.
-      + eapply wf_ext_consistent; eauto.
-Qed.
-
-
 Program Definition referenced_pop {cf:checker_flags} (Σ : referenced_impl) : referenced_impl :=
 match Σ.(declarations) with
  [] => Σ
@@ -108,29 +47,28 @@ Program Definition make_wf_env_ext {cf:checker_flags} {guard : abstract_guard_im
 
 Program Global Instance canonical_abstract_env_struct {cf:checker_flags} {guard : abstract_guard_impl} :
   abstract_env_struct referenced_impl referenced_impl_ext :=
-  {| abstract_env_lookup := fun Σ => lookup_env (referenced_impl_env_ext Σ) ;
-     abstract_env_conv_pb_relb := fun Σ conv_pb => conv_pb_relb (referenced_impl_ext_graph Σ) conv_pb ;
-     abstract_env_level_mem := fun Σ levels l => LevelSet.mem l (LevelSet.union levels (global_ext_levels (referenced_impl_env_ext Σ)));
-     abstract_env_ext_wf_universeb := fun Σ u => wf_universeb Σ u;
-     abstract_env_check_constraints := fun Σ => check_constraints (referenced_impl_ext_graph Σ);
-
-     abstract_env_guard := fun Σ fix_cofix => guard_impl fix_cofix (referenced_impl_env_ext Σ);
-     abstract_env_ext_rel := fun X Σ => Σ = referenced_impl_env_ext X;
- abstract_env_init := fun cs retro H =>  {|
- referenced_impl_env := {| universes := cs ; declarations := []; retroknowledge := retro |};
- |} ;
- abstract_env_add_decl := fun X kn d H =>
-  {| referenced_impl_env := add_global_decl X.(referenced_impl_env) (kn,d);
-   |};
- abstract_env_is_consistent X uctx :=
+  {|
+  abstract_env_lookup := fun Σ => lookup_env (referenced_impl_env_ext Σ) ;
+  abstract_env_leqb_level_n := fun Σ => leqb_level_n (referenced_impl_ext_graph Σ) ;
+  abstract_env_level_mem := fun Σ levels l => LevelSet.mem l (LevelSet.union levels (global_ext_levels (referenced_impl_env_ext Σ)));
+  abstract_env_ext_wf_universeb := fun Σ u => wf_universeb Σ u;
+  abstract_env_guard := fun Σ fix_cofix => guard_impl fix_cofix (referenced_impl_env_ext Σ);
+  abstract_env_ext_rel := fun X Σ => Σ = referenced_impl_env_ext X;
+  abstract_env_init := fun cs retro H =>  {|
+     referenced_impl_env := {| universes := cs ;
+                               declarations := [];
+                               retroknowledge := retro |}; |} ;
+  abstract_env_add_decl := fun X kn d H =>
+    {| referenced_impl_env := add_global_decl X.(referenced_impl_env) (kn,d); |};
+  abstract_env_is_consistent X uctx :=
    let G := referenced_impl_graph X in
    let G' := add_uctx uctx G in
    wGraph.is_acyclic G' && wGraph.IsFullSubgraph.is_full_extension G G' ;
- abstract_env_add_udecl X udecl Hglobal := {| referenced_impl_env_ext := (X.(referenced_impl_env) , udecl);
- |} ;
- abstract_primitive_constant := fun X tag => primitive_constant X tag;
- abstract_env_rel := fun X Σ => Σ = referenced_impl_env X ;
- abstract_pop_decls := referenced_pop ;
+  abstract_env_add_udecl X udecl Hglobal :=
+    {| referenced_impl_env_ext := (X.(referenced_impl_env) , udecl); |} ;
+  abstract_primitive_constant := fun X tag => primitive_constant X tag;
+  abstract_env_rel := fun X Σ => Σ = referenced_impl_env X ;
+  abstract_pop_decls := referenced_pop ;
  |}.
 Next Obligation. sq; constructor; cbn; eauto. econstructor. Qed.
 Next Obligation.
@@ -237,10 +175,9 @@ Program Global Instance optimized_abstract_env_struct {cf:checker_flags} {guard 
   abstract_env_struct wf_env wf_env_ext :=
  {|
  abstract_env_lookup := fun Σ k => EnvMap.lookup k (wf_env_ext_map Σ);
- abstract_env_conv_pb_relb X := abstract_env_conv_pb_relb X.(wf_env_ext_referenced);
+ abstract_env_leqb_level_n X := abstract_env_leqb_level_n X.(wf_env_ext_referenced);
  abstract_env_level_mem X := abstract_env_level_mem X.(wf_env_ext_referenced);
  abstract_env_ext_wf_universeb X := abstract_env_ext_wf_universeb X.(wf_env_ext_referenced);
- abstract_env_check_constraints X := abstract_env_check_constraints X.(wf_env_ext_referenced);
  abstract_env_guard := fun Σ fix_cofix => guard_impl fix_cofix (wf_env_ext_referenced Σ);
  abstract_env_ext_rel X := abstract_env_ext_rel X.(wf_env_ext_referenced);
 
@@ -260,7 +197,7 @@ Next Obligation.
   pose proof (X.(wf_env_referenced).(referenced_impl_wf)) as [?].
   sq. destruct (H _ eq_refl).
   apply EnvMap.repr_add; eauto; try eapply wf_fresh_globals; eauto.
-  destruct X1; eauto. 
+  destruct X1; eauto.
   apply wf_env_map_repr.
 Qed.
 Next Obligation. apply wf_env_map_repr. Qed.
@@ -327,28 +264,6 @@ Section GraphSpec.
     destruct HΣ, Hφ; now constructor.
   Qed.
 
-  Lemma check_constraints_spec ctrs
-    : check_constraints G ctrs -> valid_constraints (global_ext_constraints Σ) ctrs.
-  Proof using HG HΣ Hφ.
-    pose proof HΣ'.
-    intros HH.
-    refine (check_constraints_spec G (global_ext_uctx Σ) _ _ HG _ HH).
-    sq; now eapply wf_ext_global_uctx_invariants.
-    sq; now eapply global_ext_uctx_consistent.
-  Qed.
-
-  Lemma check_constraints_complete ctrs (H : check_univs) :
-  uctx_invariants ((global_ext_uctx Σ).1, ctrs) -> valid_constraints (global_ext_constraints Σ) ctrs -> check_constraints G ctrs.
-  Proof.
-    pose proof HΣ'.
-    intros Huctx HH.
-    refine (check_constraints_complete G (global_ext_uctx Σ) _ _ HG _ _ _ HH); eauto; sq.
-    now eapply wf_ext_global_uctx_invariants.
-    now eapply global_ext_uctx_consistent.
-    pose proof (wf_ext_global_uctx_invariants Σ H0) as [H1 H2].
-    split; eauto.
-  Qed.
-
   Lemma is_graph_of_uctx_levels (l : Level.t) :
     LevelSet.mem l (uGraph.wGraph.V G) <->
     LevelSet.mem l (global_ext_levels Σ).
@@ -369,33 +284,44 @@ Program Global Instance canonical_abstract_env_prop {cf:checker_flags} {guard : 
   @abstract_env_prop _ _ _ canonical_abstract_env_struct :=
      {| abstract_env_ext_exists := fun Σ => sq (referenced_impl_env_ext Σ ; eq_refl); |}.
 Next Obligation. wf_env. Qed.
-Next Obligation. apply check_conv_pb_relb_correct; eauto; wf_env.
-   apply (graph_of_wf_ext X).π2. Qed.
-Next Obligation. split; intros.
-  - eapply check_constraints_complete; eauto.
-    apply referenced_impl_sq_wf. apply Σudecl_ref.
-    apply (graph_of_wf_ext X).π2.
-    now destruct X.
-  - eapply check_constraints_spec; eauto.
-  apply referenced_impl_sq_wf. apply Σudecl_ref.
-  apply (graph_of_wf_ext X).π2.
-  Qed.
+Next Obligation.
+  pose proof (referenced_impl_ext_wf X); sq.
+  set (uctx := wf_ext_gc_of_uctx _); destruct uctx as [[l ctrs] Huctx].
+  assert (consistent (global_ext_uctx X).2) as HC.
+      { sq; apply (global_ext_uctx_consistent _ H). }
+  simpl in HC. apply gc_consistent_iff in HC.
+  split.
+  - eapply leqb_level_n_spec0.
+    + eapply gc_of_uctx_invariants; try eapply wf_ext_global_uctx_invariants; eauto.
+    + Opaque gc_of_constraints. cbn in *. Transparent gc_of_constraints.
+      destruct (gc_of_constraints X); inversion Huctx. now destruct H2.
+    + unfold referenced_impl_ext_graph; cbn.
+      set (G := graph_of_wf_ext _); destruct G as [G HG].
+      cbn. unfold is_graph_of_uctx in HG. now rewrite Huctx in HG.
+  - eapply leqb_level_n_spec.
+    + eapply gc_of_uctx_invariants; try eapply wf_ext_global_uctx_invariants; eauto.
+    + Opaque gc_of_constraints. cbn in *. Transparent gc_of_constraints.
+      destruct (gc_of_constraints X); inversion Huctx. now destruct H2.
+    + unfold referenced_impl_ext_graph; cbn.
+      set (G := graph_of_wf_ext _); destruct G as [G HG].
+      cbn. unfold is_graph_of_uctx in HG. now rewrite Huctx in HG.
+Qed.
 Next Obligation. apply guard_correct. Qed.
 Next Obligation. now sq. Qed.
 Next Obligation. wf_env. Qed.
 Next Obligation. now split. Qed.
 Next Obligation.
-  rename H2 into Hudecl. unfold referenced_impl_graph; rewrite andb_and.  
+  rename H2 into Hudecl. unfold referenced_impl_graph; rewrite andb_and.
   pose proof (referenced_impl_graph_wf X) as HG.
   set (gph := (graph_of_wf X).π1) in *. clearbody gph. simpl in HG.
   pose proof (HG' := is_graph_of_uctx_add Hudecl HG).
-  pose (global_ext_uctx := ContextSet.union udecl (global_uctx X)). 
+  pose (global_ext_uctx := ContextSet.union udecl (global_uctx X)).
   rewrite - (is_consistent_spec global_ext_uctx) (is_consistent_spec2 HG').
   assert (reorder : forall a b c : Prop, (a -> b <-> c) -> a /\ b <-> a /\ c) by intuition; apply reorder.
   move=> ?; rewrite consistent_extension_on_union.
   1:{ pose proof (referenced_impl_wf X); sq.
       apply: PCUICUnivSubstitutionConv.levels_global_constraint. }
-  cbn. 
+  cbn.
   change (CS.union _ _) with global_ext_uctx.2.
   apply: consistent_ext_on_full_ext=> //.
   apply: add_uctx_subgraph.
@@ -408,18 +334,19 @@ Qed.
 Program Global Instance optimized_abstract_env_prop {cf:checker_flags} {guard : abstract_guard_impl} :
   @abstract_env_prop _ _ _ optimized_abstract_env_struct :=
      {| abstract_env_ext_exists := fun Σ => sq (referenced_impl_env_ext Σ ; eq_refl); |}.
-  Next Obligation. wf_env. Qed.
-  Next Obligation. pose (referenced_impl_ext_wf X). sq.
+Next Obligation. wf_env. Qed.
+Next Obligation. pose (referenced_impl_ext_wf X). sq.
     erewrite EnvMap.lookup_spec; try reflexivity.
     1: apply wf_fresh_globals; eauto.
     1: apply wf_env_ext_map_repr. Qed.
-  Next Obligation. now rewrite (abstract_env_compare_universe_correct X.(wf_env_ext_referenced)). Qed.
-  Next Obligation. now rewrite (abstract_env_check_constraints_correct X.(wf_env_ext_referenced)); eauto. Qed.
-  Next Obligation. eapply guard_correct. Qed.
-  Next Obligation. now sq. Qed.
+Next Obligation.
+    epose (prf := abstract_env_leqb_level_n_correct X.(wf_env_ext_referenced) eq_refl).
+    erewrite wf_ext_gc_of_uctx_irr.  exact prf. Qed.
+Next Obligation. eapply guard_correct. Qed.
+Next Obligation. now sq. Qed.
 Next Obligation. wf_env. Qed.
 Next Obligation. now split. Qed.
-Next Obligation. 
+Next Obligation.
   now erewrite (abstract_env_is_consistent_correct X.(wf_env_referenced)); eauto. Qed.
 Next Obligation. unfold optim_pop. set (optim_pop_obligation_1 cf X). clearbody r.
   pose proof (reference_pop_decls_correct X decls prf X (referenced_pop X) eq_refl eq_refl).
